src/Solver/RSolver.dfy
@@ -1,0 +1,84 @@
+module RSolvers {
+  import SolverExpr
+  import Solvers
+  import Z3SmtSolver
+
+  export
+    provides RSolver, RSolver.Repr, RSolver.Valid
+    provides Create
+    provides RSolver.Extend, RSolver.Prove, RSolver.Record
+    reveals RExpr
+    provides RExpr.Eq
+    provides SolverExpr, Solvers
+
+  method Create() returns (r: RSolver)
+    ensures r.Valid() && fresh(r.Repr())
+  {
+    var z3 := Z3SmtSolver.CreateZ3Solver();
+    var state := new Solvers.SolverState(z3);
+    var solver := Solvers.Solver.Empty();
+    return RSolver(solver, state);
+  }
+
+  datatype RExpr =
+    | Boolean(b: bool)
+    | Integer(x: int)
+    | Id(v: SolverExpr.SVar)
+    | FuncAppl(op: string, args: seq<RExpr>)
+  {
+    function ToSExpr(): SolverExpr.SExpr {
+      match this
+      case Boolean(b) => SolverExpr.SExpr.Boolean(b)
+      case Integer(x) => SolverExpr.SExpr.Integer(x)
+      case Id(v) => SolverExpr.SExpr.Id(v)
+      case FuncAppl(op, args) => SolverExpr.SExpr.FuncAppl(op, seq(|args|, i requires 0 <= i < |args| => args[i].ToSExpr()))
+    }
+
+    static function Eq(r0: RExpr, r1: RExpr): RExpr {
+      FuncAppl("=", [r0, r1])
+    }
+  }
+
+  datatype RSolver = RSolver(solver: Solvers.Solver, state: Solvers.SolverState)
+  {
+    function Repr(): set<object> {
+      { state, state.solver, state.solver.process }
+    }
+
+    ghost predicate Valid()
+      reads Repr()
+    {
+      state.Valid() && state.ValidFor(solver)
+    }
+
+    method Extend(expr: RExpr) returns (r: RSolver)
+      requires Valid()
+      modifies Repr()
+      ensures r.Valid() && r.Repr() == Repr()
+    {
+      var solver := this.solver;
+      // TODO: declare the new symbols in "expr"
+      solver := solver.Extend(expr.ToSExpr(), state);
+      return RSolver(solver, state);
+    }
+
+    method Prove(expr: RExpr)
+      requires Valid()
+      modifies Repr()
+      ensures Valid()
+    {
+      // TODO: declare the new symbols in "expr"
+      solver.Prove(expr.ToSExpr(), state);
+    }
+
+    method Record(expr: RExpr) returns (r: RSolver)
+      requires Valid()
+      modifies Repr()
+      ensures r.Valid() && r.Repr() == Repr()
+    {
+      // TODO: declare the new symbols in "expr"
+      var solver := solver.Record(expr.ToSExpr());
+      return RSolver(solver, state);
+    }
+  }
+}
